progress on proof

ArkLib/CommitmentScheme/InductiveMerkleTree.lean
@@ -17,15 +17,51 @@ This file implements Merkle Trees. In contrast to the other Merkle tree implemen
 
 ## Notes & TODOs
 
+### Binary Tree API
+
+- Split this BinaryTree API to a new file
+- More API about equivlances between
+  - `SkeletonNodeIndex` ≃ `SkeletonInternalIndex` ⊕ `SkeletonLeafIndex`
+  - analogously
+  - `FullDataTree α ≃ InternalDataTree α × LeafDataTree α`
+  - OR EVEN BETTER:
+    - Redefine `FullDataTree`, `InternalDataTree`, `LeafDataTree` in terms of functions from `Skeleton`, so that this equivalence follows immediately from the above by algebra.
+- Replace `List`s with `FreeSubgroup` for ancestors?
+- Functions for navigating tree
+  - [ ] Go to parent if it exists
+  - [ ] Go to left child if it exists
+  - [ ] Go to right child if it exists
+  - [ ] Go to sibling if it exists
+  - [ ] Return Sym2 of left and right children
+  - Function for relationships between all these tree navigations
+    - [ ] How do these navigations affect depth?
+    - [ ] Which navigation sequences are equivalent to each other?
+- API for functorial mapping over data carried by the tree
+- API for flatttening a tree to a list
+- Define `Lattice` strutcure of trees
+  - a susbset relation on trees, mappings of indices to indices of supertrees
+- Define a datatype for indices of general trees, equivalent to lists of bools, and relationships to normal types.
+
+### More Things needed for basic Merkle Trees
+
+- Collision Lemma (See SNARGs book 18.3)
+  - (this is really not a lemma about oracles, so it could go with the binary tree API)
+
+### More Complicated Merkle Trees
+
 We want this treatment to be as comprehensive as possible. In particular, our formalization
 should (eventually) include all complexities such as the following:
 
 - Multi-instance extraction & simulation
 - Dealing with arbitrary trees (may have arity > 2, or is not complete)
-- Path pruning optimization
+- Path pruning optimization for multi-leaf proofs
+
+
+
 -/
 
 namespace BinaryTree
+#check Lattice
 
 /-!
 # Binary Trees
@@ -79,6 +115,25 @@ def SkeletonNodeIndex.depth {s : Skeleton} : SkeletonNodeIndex s → Nat
   | SkeletonNodeIndex.ofLeft idxLeft => idxLeft.depth + 1
   | SkeletonNodeIndex.ofRight idxRight => idxRight.depth + 1
 
+def SkeletonNodeIndex.parent {s : Skeleton} (idx : SkeletonNodeIndex s) : Option (SkeletonNodeIndex s) :=
+  match idx with
+  | SkeletonNodeIndex.ofLeaf => none
+  | SkeletonNodeIndex.ofInternal => none
+  | SkeletonNodeIndex.ofLeft (.ofLeaf) => some .ofInternal
+  | SkeletonNodeIndex.ofLeft (.ofInternal) => some .ofInternal
+  | SkeletonNodeIndex.ofLeft idxLeft =>
+    idxLeft.parent.map (SkeletonNodeIndex.ofLeft)
+  | SkeletonNodeIndex.ofRight (.ofLeaf) => some .ofInternal
+  | SkeletonNodeIndex.ofRight (.ofInternal) => some .ofInternal
+  | SkeletonNodeIndex.ofRight idxRight =>
+    idxRight.parent.map (SkeletonNodeIndex.ofRight)
+
+/-- Get the root value of a InternalDataTree. -/
+def getRootIndex (s : Skeleton) : SkeletonNodeIndex s := match s with
+  | Skeleton.leaf => SkeletonNodeIndex.ofLeaf
+  | Skeleton.internal left right =>
+    SkeletonNodeIndex.ofInternal
+
 -- Analogous to `Cache`
 /--
 A binary tree with values stored in internal nodes.
@@ -99,6 +154,15 @@ inductive LeafDataTree (α : Type) : Skeleton → Type
       LeafDataTree α (Skeleton.internal left right)
   deriving Repr
 
+/-- Get the root value of a InternalDataTree. -/
+def LeafDataTree.getValueAtIndex {s} {α : Type} (tree : LeafDataTree α s) (idx : SkeletonLeafIndex s) : α :=
+  match tree, idx with
+  | LeafDataTree.leaf value, SkeletonLeafIndex.ofLeaf => value
+  | LeafDataTree.internal left right, SkeletonLeafIndex.ofLeft idxLeft =>
+    LeafDataTree.getValueAtIndex left idxLeft
+  | LeafDataTree.internal left right, SkeletonLeafIndex.ofRight idxRight =>
+    LeafDataTree.getValueAtIndex right idxRight
+
 /--
 A binary tree with values stored at both leaves and internal nodes.
 -/
@@ -110,23 +174,20 @@ inductive FullDataTree (α : Type) : Skeleton → Type
       FullDataTree α (Skeleton.internal left right)
 
 /-- Get the root value of a InternalDataTree. -/
-def getRoot {s} {α : Type} : FullDataTree α s → α
-  | FullDataTree.leaf value => value
-  | FullDataTree.internal value _ _ => value
+def FullDataTree.getValueAtIndex {s} {α : Type} (tree : FullDataTree α s) (idx : SkeletonNodeIndex s) : α :=
+  match tree, idx with
+  | FullDataTree.leaf value, SkeletonNodeIndex.ofLeaf => value
+  | FullDataTree.internal value _ _, SkeletonNodeIndex.ofInternal => value
+  | FullDataTree.internal _ left right, SkeletonNodeIndex.ofLeft idxLeft =>
+    FullDataTree.getValueAtIndex left idxLeft
+  | FullDataTree.internal _ left right, SkeletonNodeIndex.ofRight idxRight =>
+    FullDataTree.getValueAtIndex right idxRight
 
--- TODO not sure I got this right
-def SkeletonNodeIndex.parent {s : Skeleton} (idx : SkeletonNodeIndex s) : Option (SkeletonNodeIndex s) :=
-  match idx with
-  | SkeletonNodeIndex.ofLeaf => none
-  | SkeletonNodeIndex.ofInternal => none
-  | SkeletonNodeIndex.ofLeft (.ofLeaf) => some .ofInternal
-  | SkeletonNodeIndex.ofLeft (.ofInternal) => some .ofInternal
-  | SkeletonNodeIndex.ofLeft idxLeft =>
-    idxLeft.parent.map (SkeletonNodeIndex.ofLeft)
-  | SkeletonNodeIndex.ofRight (.ofLeaf) => some .ofInternal
-  | SkeletonNodeIndex.ofRight (.ofInternal) => some .ofInternal
-  | SkeletonNodeIndex.ofRight idxRight =>
-    idxRight.parent.map (SkeletonNodeIndex.ofRight)
+
+/-- Get the root value of a InternalDataTree. -/
+def FullDataTree.getRootValue {s} {α : Type} (tree : FullDataTree α s) :=
+  tree.getValueAtIndex (getRootIndex s)
+
 
 lemma SkeletonNodeIndex.parent_of_depth_zero {s : Skeleton} (idx : SkeletonNodeIndex s) (h : idx.depth = 0) :
     parent idx = none := by
@@ -140,30 +201,101 @@ lemma SkeletonNodeIndex.parent_of_depth_zero {s : Skeleton} (idx : SkeletonNodeI
     unfold depth at h
     simp_all
 
+
+
 lemma SkeletonNodeIndex.parent_of_depth_succ {s : Skeleton} (idx : SkeletonNodeIndex s) (n : ℕ) (h : idx.depth = n + 1) :
     idx.parent.map depth = some n := by
-  cases idx with
-  | ofLeaf => sorry
-  | ofInternal => sorry
-  | ofLeft idxLeft => sorry
-  | ofRight idxRight => sorry
+  sorry
+  -- cases idx with
+  -- | ofLeaf =>
+  --   unfold depth at h
+  --   exfalso
+  --   omega
+  -- | ofInternal =>
+  --   unfold depth at h
+  --   exfalso
+  --   omega
+  -- | ofLeft idxLeft =>
+  --   cases idxLeft with
+  --   | ofLeaf =>
+  --     unfold depth at h
+  --     unfold depth at h
+  --     unfold parent
+  --     unfold Option.map
+  --     unfold depth
+  --     simp_all
+  --   | ofInternal =>
+  --     unfold depth at h
+  --     unfold depth at h
+  --     unfold parent
+  --     unfold Option.map
+  --     unfold depth
+  --     simp_all
+  --   | ofLeft idxLeftLeft =>
+  --     unfold depth at h
+  --     unfold depth at h
+  --     unfold parent
+  --     rw [Option.map_map]
+  --     unfold Option.map
+  --     cases idxLeftLeft.ofLeft.parent with
+  --     | none =>
+  --       simp_all
+  --       sorry
+  --     | some idxLeftLeftParent =>
+  --       sorry
+  --     -- unfold depth
+  --     simp_all
+  --   | ofRight idxLeftRight => sorry
+  -- | ofRight idxRight => sorry
+
 
 /--
-Given a `Skeleton`, and a node index of the skeleton, return a list of node indices which are the ancestors of the node.
+Given a `Skeleton`, and a node index of the skeleton,
+return a list of node indices which are the ancestors of the node, starting with the root node, working down to the node itself.
 -/
 def SkeletonNodeIndex.findAncestors {s : Skeleton} (idx : SkeletonNodeIndex s) : List (SkeletonNodeIndex s) :=
-  idx ::
+  match idx with
+  | SkeletonNodeIndex.ofLeaf => [SkeletonNodeIndex.ofLeaf]
+  | SkeletonNodeIndex.ofInternal => [SkeletonNodeIndex.ofInternal]
+  | SkeletonNodeIndex.ofLeft idxLeft =>
+    .ofInternal :: ((idxLeft.findAncestors)).map (SkeletonNodeIndex.ofLeft)
+  | SkeletonNodeIndex.ofRight idxRight =>
+    .ofInternal :: ((idxRight.findAncestors)).map (SkeletonNodeIndex.ofRight)
 
 /--
 Given a `Skeleton`, and a leaf index of the skeleton, return a list of node indices which are the ancestors of the leaf.
 -/
 def findAncestors {s : Skeleton} (idx : SkeletonLeafIndex s) : List (SkeletonNodeIndex s) :=
+  SkeletonNodeIndex.findAncestors idx.toNodeIndex
+
+/--
+Return the sibling node index of a given `SkeletonNodeIndex`. Or `none` if the node is the root
+-/
+def SkeletonNodeIndex.findSibling {s : Skeleton} (idx : SkeletonNodeIndex s) : Option (SkeletonNodeIndex s) :=
   match idx with
-  | SkeletonLeafIndex.ofLeaf => .ofLeaf :: []
-  | SkeletonLeafIndex.ofLeft idxLeft =>
-    (idxLeft.toNodeIndex :: (findAncestors idxLeft)).map (SkeletonNodeIndex.ofLeft)
-  | SkeletonLeafIndex.ofRight idxRight =>
-    idxRight.toNodeIndex.ofRight :: (findAncestors idxRight).map (SkeletonNodeIndex.ofRight)
+  | SkeletonNodeIndex.ofLeaf => none
+  | SkeletonNodeIndex.ofInternal => none
+  | @SkeletonNodeIndex.ofLeft left right idxLeft =>
+    match idxLeft with
+    | SkeletonNodeIndex.ofLeaf => some (getRootIndex right).ofRight
+    | SkeletonNodeIndex.ofInternal => some (getRootIndex right).ofRight
+    | SkeletonNodeIndex.ofLeft idxLeftLeft =>
+      idxLeftLeft.ofLeft.findSibling.map (SkeletonNodeIndex.ofLeft)
+    | SkeletonNodeIndex.ofRight idxLeftRight =>
+      idxLeftRight.ofRight.findSibling.map (SkeletonNodeIndex.ofLeft)
+  | @SkeletonNodeIndex.ofRight left right idxRight =>
+    match idxRight with
+    | SkeletonNodeIndex.ofLeaf => some (getRootIndex left).ofLeft
+    | SkeletonNodeIndex.ofInternal => some (getRootIndex left).ofLeft
+    | SkeletonNodeIndex.ofLeft idxRightLeft =>
+      idxRightLeft.ofLeft.findSibling.map (SkeletonNodeIndex.ofRight)
+    | SkeletonNodeIndex.ofRight idxRightRight =>
+      idxRightRight.ofRight.findSibling.map (SkeletonNodeIndex.ofRight)
+
+/-- Find the siblings of the ancestors of a node -/
+def SkeletonNodeIndex.findUncles {s : Skeleton} (idx : SkeletonNodeIndex s) :
+    List (SkeletonNodeIndex s) := (idx.findAncestors.filterMap (fun idx => idx.findSibling))
+
 
 end BinaryTree
 
@@ -224,42 +356,127 @@ variable {α : Type}
 --     | none => getProofHelper rest r
 --     | some v => v :: getProofHelper rest r
 
-def buildMerkleTree_with_hash (leaf_tree : LeafTree α) (hashFn : α → α → α) : (BinaryTree α) :=
+def buildMerkleTree_with_hash {s} (leaf_tree : LeafDataTree α s) (hashFn : α → α → α) : (FullDataTree α s) :=
   match leaf_tree with
-  | LeafTree.leaf a => BinaryTree.node a none
-  | LeafTree.node left right =>
+  | LeafDataTree.leaf a => FullDataTree.leaf a
+  | LeafDataTree.internal left right =>
     let leftTree := buildMerkleTree_with_hash left hashFn
     let rightTree := buildMerkleTree_with_hash right hashFn
-    let root_hash := hashFn (getRoot leftTree) (getRoot rightTree)
-    BinaryTree.node root_hash (some (leftTree, rightTree))
+    let rootHash := hashFn (leftTree.getRootValue) (rightTree.getRootValue)
+    FullDataTree.internal rootHash leftTree rightTree
 
 /-- Build the full Merkle tree, returning the cache -/
-def buildMerkleTree (leaf_tree : LeafTree α) : OracleComp (spec α) (BinaryTree α) :=
+def buildMerkleTree {s} (leaf_tree : LeafDataTree α s) : OracleComp (spec α) (FullDataTree α s) :=
   match leaf_tree with
-  | LeafTree.leaf a => do
-    return BinaryTree.node a none
-  | LeafTree.node left right => do
+  | LeafDataTree.leaf a => do return (FullDataTree.leaf a)
+  | LeafDataTree.internal left right => do
     let leftTree ← buildMerkleTree left
     let rightTree ← buildMerkleTree right
-    let rootHash ← singleHash α (getRoot leftTree) (getRoot rightTree)
-    return BinaryTree.node rootHash (some (leftTree, rightTree))
+    let rootHash ← singleHash α leftTree.getRootValue rightTree.getRootValue
+    return FullDataTree.internal rootHash leftTree rightTree
 
-/-- Generate a Merkle proof for a leaf with value 'a'.
-    The proof consists of the sibling hashes needed to recompute the root. -/
-def generateProof [DecidableEq α] (a : α) (tree : BinaryTree α) : Option (List α) :=
-  match findPath a tree with
-  | none => none
-  | some path => some (getProofHelper path tree)
+/-- Generate a Merkle proof for a leaf at a given idx
+    The proof consists of the sibling hashes needed to recompute the root.
 
-/-- Verify a Merkle proof that a value 'a' is in the tree with root 'root'.
-    The 'proof' contains sibling hashes, and 'path' is the position (left/right) at each level. -/
-def verifyProof [DecidableEq α] (hashFn : α → α → α) (a : α) (root : α)
-    (proof : List α) (path : List Bool) : Bool :=
-  let rec verify (current : α) (p : List α) (dirs : List Bool) : Bool :=
-    match p, dirs with
-    | [], [] => current = root
-    | sibling :: restProof, dir :: restPath =>
-      let nextHash := if dir then hashFn sibling current else hashFn current sibling
-      verify nextHash restProof restPath
-    | _, _ => false -- Proof and path lengths don't match
-  verify a proof path
+-/
+def generateProof {s} (cache_tree : FullDataTree α s) (idx : BinaryTree.SkeletonLeafIndex s) : List α :=
+  (idx.toNodeIndex.findUncles.map (fun siblingIdx =>
+    cache_tree.getValueAtIndex siblingIdx))
+
+/--
+Given a leaf index, a leaf value at that index, and putative proof,
+returns the hash that would be the root of the tree if the proof was valid.
+i.e. the hash obtained by combining the leaf in sequence with each member of the proof,
+according to its index.
+-- TODO should this, instead of a List, take a Vector of length idx.depth?
+-/
+def getPutativeRoot {s} (idx : BinaryTree.SkeletonLeafIndex s) (leafValue : α)
+    (proof : List α) : OracleComp (spec α) α :=
+  match proof with
+  | [] => return leafValue -- If no proof, the root is just the leaf value
+  | siblingBelowRootHash :: restProof => do
+    match idx with
+    | BinaryTree.SkeletonLeafIndex.ofLeaf =>
+      -- This indicates that the proof is longer than the depth of the tree, which is invalid.
+      -- A more well-typed version using `Vector` might prevent this.
+      -- FOr now, we just return the leaf value.
+      return leafValue
+    | BinaryTree.SkeletonLeafIndex.ofLeft idxLeft =>
+      -- Recursively get the hash of the ancestor of the leaf which is just below the root
+      let ancestorBelowRootHash ← getPutativeRoot idxLeft leafValue restProof
+      singleHash α ancestorBelowRootHash siblingBelowRootHash
+    | BinaryTree.SkeletonLeafIndex.ofRight idxRight =>
+      -- Recursively get the hash of the ancestor of the leaf which is just below the root
+      let ancestorBelowRootHash ← getPutativeRoot idxRight leafValue restProof
+      singleHash α siblingBelowRootHash ancestorBelowRootHash
+
+/-- Verify a Merkle proof `proof` that a given `leaf` at index `i` is in the Merkle tree with given
+  `root`.
+  Works by computing the putative root based on the branch, and comparing that to the actual root.
+  Outputs `failure` if the proof is invalid. -/
+def verifyProof [DecidableEq α] {s} (idx : BinaryTree.SkeletonLeafIndex s) (leafValue : α) (rootValue : α)
+    (proof : List α) : OracleComp (spec α) Unit := do
+  let putative_root ← getPutativeRoot idx leafValue proof
+  guard (putative_root = rootValue)
+
+theorem singleHash_neverFails [DecidableEq α] [inst_1 : SelectableType α] (left right : α)
+    (preexisting_cache : (spec α).QueryCache) :
+    ((simulateQ randomOracle (singleHash α left right)).run preexisting_cache).neverFails := by
+  unfold singleHash
+  simp only [range_def, bind_pure, simulateQ_query,
+    unifOracle.apply_eq, StateT.run_bind, StateT.run_get, pure_bind]
+  simp
+  cases preexisting_cache () (left, right) with
+  | none =>
+    simp only [StateT.run_bind, StateT.run_monadLift, monadLift_self, bind_pure_comp,
+      StateT.run_modifyGet, Functor.map_map, neverFails_map_iff, neverFails_uniformOfFintype]
+  | some u =>
+    simp only [StateT.run_pure, neverFails_pure]
+
+theorem buildMerkleTree_neverFails {α : Type} [inst : DecidableEq α] [inst_1 : SelectableType α] {s : Skeleton}
+    (leaf_tree : LeafDataTree α s) (preexisting_cache : (spec α).QueryCache) :
+    ((simulateQ randomOracle (buildMerkleTree leaf_tree)).run preexisting_cache).neverFails := by
+  induction leaf_tree generalizing preexisting_cache with
+  | leaf a =>
+    unfold buildMerkleTree
+    simp only [simulateQ_pure, StateT.run_pure, neverFails_pure]
+  | internal left right left_ih right_ih =>
+    unfold buildMerkleTree
+    simp [simulateQ_bind, StateT.run_bind, neverFails_bind_iff, left_ih, right_ih]
+    intro merkle_cache_left query_cache h_mem_support merkle_cache_right query_cache' h_mem_support'
+    clear left_ih right_ih
+    exact
+      singleHash_neverFails merkle_cache_left.getRootValue merkle_cache_right.getRootValue
+        query_cache'
+
+theorem completeness [DecidableEq α] [SelectableType α] {s} (leaf_tree : LeafDataTree α s) (idx : BinaryTree.SkeletonLeafIndex s)
+    (preexisting_cache : (spec α).QueryCache) :
+    (((do
+      let cache ← buildMerkleTree leaf_tree
+      let proof := generateProof cache idx
+      let verif ← verifyProof idx (leaf_tree.getValueAtIndex idx) (cache.getRootValue) proof).simulateQ
+      (randomOracle)).run preexisting_cache).neverFails := by
+  simp [neverFails_bind_iff]
+  constructor
+  · -- buildMerkleTree never fails
+    exact buildMerkleTree_neverFails leaf_tree preexisting_cache
+  · -- verifyProof never fails on the output of generateProof after buildMerkleTree
+    intros merkle_tree_cache query_cache h_mem_support
+    -- Need a theorem to characterize
+    -- `(merkle_tree_cache, query_cache) ∈ ((simulateQ randomOracle (buildMerkleTree leaf_tree)).run preexisting_cache).support`
+    -- i.e. this is equivalent to:
+    --  - All merkle_tree_cache parent-child relationships are in the query_cache
+    --  - Everything in the preexisting_cache is in the query_cache (so merkle_tree_cache and preexisting_cache are compatible)
+    --  - Nothing else is in the query_cache
+    simp [verifyProof, neverFails_bind_iff]
+    constructor
+    · -- getPutativeRoot never fails
+      sorry
+    · -- guard never fails
+      intro putative_root query_cache' h_mem_support'
+      -- Now, Need a theorem to characterize
+      -- `(putative_root, query_cache') ∈ ((simulateQ randomOracle
+      --     (getPutativeRoot idx (leaf_tree.getValueAtIndex idx) (generateProof merkle_tree_cache idx))).run
+      -- query_cache✝).support`
+
+      sorry
